src/equiv/TsoPFtoA.v
@@ -207,7 +207,6 @@ Proof.
         { apply Loc.cl_refl. }
         ii. inv EID. inv REL. obtac. inv_po.
       + ii. inv EID. inv REL; obtac; inv_po.
-      + ii. inv EID. inv REL; obtac; inv_po.
       + ii. inv EID. inv REL. obtac. inv_po.
       + ii. inv EID. inv REL; obtac; inv_po.
   }
@@ -680,7 +679,7 @@ Proof.
     { s. instantiate (1 := length tr'0). lia. }
     all: try rewrite lastn_all; s; eauto; try lia.
     intro TH'.
-    eapply TH'.(LC).(PER_END). econs; eauto.
+    eapply TH'.(LC).(PER). econs; eauto.
     left. econs. split; simtac.
     econs; eauto. apply List.nth_error_Some. ss. rewrite EID2. ss.
   - (* flushopt *)
@@ -704,8 +703,8 @@ Proof.
     { s. instantiate (1 := length tr'0). lia. }
     all: try rewrite lastn_all; s; eauto; try lia.
     intro TH'.
-    eapply TH'.(LC).(PER_END). econs; eauto.
-    right. econs. split; simtac.
+    eapply TH'.(LC).(PER). econs; eauto.
+    right. econs. split; econs; simtac.
     econs; eauto. apply List.nth_error_Some. ss. rewrite EID3. ss.
 Qed.
 
